\documentclass{article}

\usepackage[leqno]{amsmath}
\usepackage{amsfonts}
\usepackage{bussproofs}

\begin{document}

\section*{Terms}

\begin{align}
\tag*{Literals} l ::=& \; true \mid false \mid Bool \mid \mathbb{R} \mid Float \mid () \mid Unit \mid Type \mid \Box \\
\tag*{Variables} v ::=& \; [a-z|A-Z][a-z|A-Z|1-9]* \\
\tag*{Expressions} e,t,k ::=& \mid l \\
\tag*{} & \mid v \\
\tag*{} & \mid \lambda v : t. e \\
\tag*{} & \mid \forall v : t. e \\
\tag*{} & \mid e_f \; e_a \\
\tag*{} & \mid if \; e_p \; then \; e_c \; else \; e_a \\
\tag*{} & \mid let \; v \; = \; e_v \; in \; e_b \\
\tag*{} & \mid letrec \;v \; : \; t \;  = e_v \; in \; e_b \\
\tag*{} & \mid (e_l, e_r) \\
\tag*{} & \mid e.L \\
\tag*{} & \mid e.R \\
\tag*{} & \mid e.R \\
\tag*{} & \mid (t_l \land t_r) \\
\tag*{} & \mid (e : t) \\
\tag*{} & \mid (e)
\end{align}

\section*{Typing}
\subsection*{Literals}

\begin{center}

  \AxiomC{}
  \RightLabel{BLit}
  \UnaryInfC{$\vdash true : Bool$}
  \DisplayProof
  \hskip 1.5em
  \AxiomC{}
  \RightLabel{BLit}
  \UnaryInfC{$\vdash false : Bool$}
  \DisplayProof
  \hskip 1.5em
  \AxiomC{}
  \RightLabel{BTLit}
  \UnaryInfC{$\vdash Bool : Type$}
  \DisplayProof
  \vskip 1.5em
  \AxiomC{}
  \RightLabel{FLit}
  \UnaryInfC{$\vdash \mathbb{R} : Float$}
  \DisplayProof
  \hskip 1.5em
  \AxiomC{}
  \RightLabel{FTLit}
  \UnaryInfC{$\vdash Float : Type$}
  \DisplayProof
  \\
  \vskip 1.5em
  \AxiomC{}
  \RightLabel{ULit}
  \UnaryInfC{$\vdash () : Unit$}
  \DisplayProof
  \hskip 1.5em
  \AxiomC{}
  \RightLabel{UTLit}
  \UnaryInfC{$\vdash Unit : Type$}
  \DisplayProof
  \\
  \vskip 1.5em
  \AxiomC{}
  \RightLabel{TLit}
  \UnaryInfC{$\vdash Type : \Box$}
  \DisplayProof

\end{center}

\subsection*{Variables}

\begin{center}

\AxiomC{}
\RightLabel{Var}
\UnaryInfC{$\Gamma, v : t \vdash v : t$}
\DisplayProof

\end{center}

\pagebreak

\subsection*{Compounds}

\begin{center}

  \AxiomC{$\Gamma \vdash t : Type$}
  \RightLabel{IsType}
  \UnaryInfC{$\Gamma \vdash t :^t Type$}
  \DisplayProof
  \hskip 1.5em
  \AxiomC{$\Gamma \vdash t : \Box$}
  \RightLabel{IsKind}
  \UnaryInfC{$\Gamma \vdash t :^t \Box$}
  \DisplayProof
  \\
  \vskip 1.5em
  \AxiomC{$\Gamma \vdash t_{uv} :^t k_{uv}$}
  \AxiomC{$t_{uv} \Downarrow t_v$}
  \AxiomC{$\Gamma , t_v : k \vdash e : t_b$}
  \RightLabel{$\lambda$I}
  \TrinaryInfC{$\Gamma \vdash (\lambda v : t_{uv}. e) : (\forall v : t_v. t_b)$}
  \DisplayProof
  \\
  \vskip 1.5em
  \AxiomC{$\Gamma \vdash e_f : (\forall v : t_a. t_b)$}
  \AxiomC{$\Gamma \vdash e_a : t_a$}
  \AxiomC{$(\lambda v : t_a. t_b) e_a \Downarrow t_o$}
  \RightLabel{$\lambda$E}
  \TrinaryInfC{$\Gamma \vdash e_f \; e_a : t_o$}
  \DisplayProof
  \\
  \vskip 1.5em
  \AxiomC{$\Gamma \vdash t_{uv} :^t k_v$}
  \AxiomC{$t_{uv} \Downarrow t_v$}
  \AxiomC{$\Gamma, v : t_v \vdash t_{ub} :^t k_b$}
  \RightLabel{$\forall$I}
  \TrinaryInfC{$\Gamma \vdash (\forall v : t_{uv}. t_{ub}) : k_b$}
  \DisplayProof
  \\
  \vskip 1.5em
  \AxiomC{$\Gamma \vdash e_p : Bool$}
  \AxiomC{$\Gamma \vdash e_c : t$}
  \AxiomC{$\Gamma \vdash e_a : t$}
  \RightLabel{If}
  \TrinaryInfC{$\Gamma \vdash (if \; e_p \; then \; e_c \; else \; e_a) : t$}
  \DisplayProof
  \\
  \vskip 1.5em
  \AxiomC{$\Gamma \vdash e_v : t_v$}
  \AxiomC{$\Gamma, v : t_v \vdash e_b : t_b$}
  \RightLabel{Let}
  \BinaryInfC{$\Gamma \vdash (let \; v \; = \; e_v \; in \; e_b) : t_b$}
  \DisplayProof
  \\
  \vskip 1.5em
  \AxiomC{$\Gamma \vdash t_{uv} : k$}
  \AxiomC{$t_{uv} \Downarrow t_v$}
  \AxiomC{$\Gamma, v : t_v \vdash e_v : t_v$}
  \AxiomC{$\Gamma, v : t_v \vdash e_b : t_b$}
  \RightLabel{Letrec}
  \QuaternaryInfC{$\Gamma \vdash (letrec \; v \; : \; t_{uv} \; = \; e_v \; in \; e_b) : t_b$}
  \DisplayProof
  \\
  \vskip 1.5em
  \AxiomC{$\Gamma \vdash e_l : t_l$}
  \AxiomC{$\Gamma \vdash e_r : t_r$}
  \RightLabel{Pair}
  \BinaryInfC{$\Gamma \vdash (e_l, e_r) : (t_l \land t_r)$}
  \DisplayProof
  \hskip 1.5em
  \AxiomC{$\Gamma \vdash t_l :^t k$}
  \AxiomC{$\Gamma \vdash t_r :^t k$}
  \RightLabel{PairT}
  \BinaryInfC{$\Gamma \vdash (t_l \land t_r) : k$}
  \DisplayProof
  \\
  \vskip 1.5em
  \AxiomC{$\Gamma \vdash e : (t_l \land t_r)$}
  \RightLabel{PairL}
  \UnaryInfC{$\Gamma \vdash e.L : t_l$}
  \DisplayProof
  \hskip 1.5em
  \AxiomC{$\Gamma \vdash e : (t_l \land t_r)$}
  \RightLabel{PairR}
  \UnaryInfC{$\Gamma \vdash e.R : t_r$}
  \DisplayProof
  \\
  \vskip 1.5em
  \AxiomC{$\Gamma \vdash t_u :^t k$}
  \AxiomC{$t_u \Downarrow t$}
  \AxiomC{$\Gamma \vdash e : t$}
  \RightLabel{Asc}
  \TrinaryInfC{$\Gamma \vdash (e : t_u) : t$}
  \DisplayProof

\end{center}

\section*{Normalization}

\begin{center}

\AxiomC{}
\RightLabel{Lit}
\UnaryInfC{$l \Downarrow l$}
\DisplayProof
\hskip 1.5em
\AxiomC{}
\RightLabel{Var}
\UnaryInfC{$v \Downarrow v$}
\DisplayProof
\\
\vskip 1.5em
\AxiomC{$t \Downarrow t'$}
\AxiomC{$e \Downarrow e'$}
\RightLabel{$\lambda$}
\BinaryInfC{$\lambda v : t. e \Downarrow \lambda v : t'. e'$}
\DisplayProof
\hskip 1.5em
\AxiomC{$t_v \Downarrow t_v'$}
\AxiomC{$t_b \Downarrow t_b'$}
\RightLabel{$\forall$}
\BinaryInfC{$\forall v : t_v. t_b \Downarrow \forall v : t_v'. t_b'$}
\DisplayProof
\\
\vskip 1.5em
\AxiomC{$e_f \Downarrow e_f'$}
\AxiomC{$e_a \Downarrow e_a'$}
\RightLabel{NeuApp}
\BinaryInfC{$e_f \; e_a \Downarrow e_f' \; e_a'$}
\DisplayProof
\\
\vskip 1.5em
\AxiomC{$e_f \Downarrow \lambda v : t. e_b$}
\AxiomC{$e_b [e_a / v] \Downarrow e_b'$}
\RightLabel{$\beta$}
\BinaryInfC{$e_f \; e_a \Downarrow e_b'$}
\DisplayProof
\\
\vskip 1.5em
\AxiomC{$e_p \Downarrow e_p'$}
\AxiomC{$e_c \Downarrow e_c'$}
\AxiomC{$e_a \Downarrow e_a'$}
\RightLabel{NeuIf}
\TrinaryInfC{$if \; e_p \; then \; e_c \; else \; e_a \Downarrow if \; e_p' \; then \; e_c' \; else \; e_a'$}
\DisplayProof
\\
\vskip 1.5em
\AxiomC{$e_p \Downarrow true$}
\AxiomC{$e_c \Downarrow e_c'$}
\RightLabel{IfT}
\BinaryInfC{$if \; e_p \; then \; e_c \; else \; e_a \Downarrow e_c'$}
\DisplayProof
\hskip 1.5em
\AxiomC{$e_p \Downarrow false$}
\AxiomC{$e_a \Downarrow e_a'$}
\RightLabel{IfF}
\BinaryInfC{$if \; e_p \; then \; e_c \; else \; e_a \Downarrow e_a'$}
\DisplayProof
\\
\vskip 1.5em
\AxiomC{$e_b[e_v / v] \Downarrow e_b'$}
\RightLabel{Let}
\UnaryInfC{$let \; v \; = \; e_v \; in \; e_b \Downarrow e_b'$}
\DisplayProof
\\
\vskip 1.5em
\AxiomC{$e_b[e_v / v] \Downarrow e_b'$}
\RightLabel{Letrec}
\UnaryInfC{$let \; v \; = \; e_v \; in \; e_b \Downarrow e_b'$}
\DisplayProof
\\
\vskip 1.5em
\AxiomC{$e_l \Downarrow e_l'$}
\AxiomC{$e_r \Downarrow e_r'$}
\RightLabel{Pair}
\BinaryInfC{$(e_l, e_r) \Downarrow (e_l', e_r')$}
\DisplayProof
\hskip 1.5em
\AxiomC{$t_l \Downarrow t_l'$}
\AxiomC{$t_r \Downarrow t_r'$}
\RightLabel{PairT}
\BinaryInfC{$(t_l \land t_r) \Downarrow (t_l' \land t_r')$}
\DisplayProof
\\
\vskip 1.5em
\AxiomC{$e \Downarrow e'$}
\RightLabel{NeuPairL}
\UnaryInfC{$e.L \Downarrow e'.L$}
\DisplayProof
\hskip 1.5em
\AxiomC{$e \Downarrow (e_l, e_r)$}
\RightLabel{PairL}
\UnaryInfC{$e.L \Downarrow e_l$}
\DisplayProof
\\
\vskip 1.5em
\AxiomC{$e \Downarrow e'$}
\RightLabel{NeuPairR}
\UnaryInfC{$e.R \Downarrow e'.R$}
\DisplayProof
\hskip 1.5em
\AxiomC{$e \Downarrow (e_l, e_r)$}
\RightLabel{PairR}
\UnaryInfC{$e.R \Downarrow e_r$}
\DisplayProof
\\
\vskip 1.5em
\AxiomC{$e \Downarrow e'$}
\RightLabel{Asc}
\UnaryInfC{$(e : t) \Downarrow e'$}
\DisplayProof

\end{center}

\end{document}
